CollapsingTowers/TwoLevelMut/SyntacticTyping/Ty.lean
@@ -18,6 +18,15 @@ def erase_ty : Ty → Ty
   | .ref τ => .ref (erase_ty τ)
 
 @[simp]
+def escape_ty : Ty → Ty
+  | .nat => .nat
+  | .arrow τa τb φ ω => .arrow (escape_ty τa) (escape_ty τb) φ (escape_meffects ω)
+  | .fragment τ => .fragment (escape_ty τ)
+  | .rep τ => .rep (escape_ty τ)
+  | .unit => .unit
+  | .ref τ => .ref (escape_ty τ)
+
+@[simp]
 def wbt : Stage → Ty → Prop
   | 𝟙, .nat => true
   | 𝟙, (.arrow τ𝕒 τ𝕓 _ _) => wbt 𝟙 τ𝕒 ∧ wbt 𝟙 τ𝕓
@@ -31,6 +40,20 @@ def wbt : Stage → Ty → Prop
   | 𝟚, (.ref τ) => wbt 𝟚 τ
   | 𝟚, _ => false
 
+lemma wbt.escape : ∀ τ, wbt 𝟚 τ → wbt 𝟙 (escape_ty τ) :=
+  by
+  intros τ Hwbt
+  induction τ
+  case nat => simp
+  case arrow IH₀ IH₁ =>
+    constructor
+    apply IH₀; apply Hwbt.right.right.left
+    apply IH₁; apply Hwbt.right.right.right
+  case fragment => nomatch Hwbt
+  case rep => nomatch Hwbt
+  case unit => simp
+  case ref IH => apply IH; apply Hwbt
+
 lemma grounded_ty.under_erase : ∀ τ, wbt 𝟚 (erase_ty τ) :=
   by
   intros τ
@@ -39,8 +62,22 @@ lemma grounded_ty.under_erase : ∀ τ, wbt 𝟚 (erase_ty τ) :=
   case arrow IH₀ IH₁ =>
     constructor; rfl
     constructor; apply grounded_meffects.under_erase
-    constructor; apply IH₀; apply IH₁
-  case fragment IH => apply IH
-  case rep IH => apply IH
+    simp [IH₀, IH₁]
+  case fragment IH => simp [IH]
+  case rep IH => simp [IH]
   case unit => simp
-  case ref IH => apply IH
+  case ref IH => simp [IH]
+
+@[simp]
+lemma erase_ty.cancel_escape : ∀ τ, erase_ty (escape_ty τ) = erase_ty τ :=
+  by
+  intros τ
+  induction τ
+  case nat => simp
+  case arrow IH₀ IH₁ =>
+    rw [escape_ty, erase_ty, erase_meffects.cancel_escape]
+    simp [IH₀, IH₁]
+  case fragment IH => simp [IH]
+  case rep IH => simp [IH]
+  case unit => simp
+  case ref IH => simp [IH]
