CollapsingTowers/TwoLevelMut/SyntacticSoundness/PresvPure.lean
@@ -1,0 +1,244 @@
+import CollapsingTowers.TwoLevelMut.SyntacticSoundness.PresvSubst
+import CollapsingTowers.TwoLevelMut.SyntacticSoundness.PresvMaping
+import CollapsingTowers.TwoLevelMut.SyntacticSoundness.PresvCtx
+
+lemma typing.escape.strengthened :
+  ∀ σ Γ e τ φ ω,
+    typing σ Γ 𝟚 e τ φ ω →
+    typing σ (escape_env Γ) 𝟙 e (escape_ty τ) φ (escape_meffects ω) :=
+  by
+  generalize HEq𝕊 : 𝟚 = 𝕊
+  intros σ Γ e τ φ ω Hτ
+  revert HEq𝕊
+  apply
+    @typing.rec σ
+      (fun Γ 𝕊 e τ φ ω (H : typing σ Γ 𝕊 e τ φ ω) => 𝟚 = 𝕊 → typing σ (escape_env Γ) 𝟙 e (escape_ty τ) φ (escape_meffects ω))
+      (fun Γ e τ φ ω (H : typing_reification σ Γ e τ φ ω) => true)
+  <;> intros
+  <;> (try contradiction)
+  <;> (try simp only [escape_meffects.union, escape_meffects.empty])
+  case fvar x _ Hbinds Hwbt HEq𝕊 =>
+    rw [← HEq𝕊] at Hwbt
+    apply typing.fvar
+    . apply escape_env.binds _ _ _ _ Hbinds
+    . apply wbt.escape _ Hwbt
+  case lam Hwbt Hclosed IH HEq𝕊 =>
+    rw [← HEq𝕊] at Hwbt
+    apply typing.lam
+    . rw [← escape_env.length, ← escape_env]
+      apply IH; apply HEq𝕊
+    . apply wbt.escape _ Hwbt
+    . rw [← escape_env.length]
+      apply Hclosed
+  case app₁ IHf IHarg HEq𝕊 =>
+    apply typing.app₁
+    . apply IHf; apply HEq𝕊
+    . apply IHarg; apply HEq𝕊
+  case lit => apply typing.lit
+  case lets Hwbt Hclosed IHb IHe HEq𝕊 =>
+    rw [← HEq𝕊] at Hwbt
+    apply typing.lets
+    . apply IHb; apply HEq𝕊
+    . rw [← escape_env.length, ← escape_env]
+      apply IHe; apply HEq𝕊
+    . apply wbt.escape _ Hwbt
+    . rw [← escape_env.length]
+      apply Hclosed
+  case unit => apply typing.unit
+  case alloc₁ IH HEq𝕊 =>
+    rw [escape_meffects.init]
+    apply typing.alloc₁
+    apply IH; apply HEq𝕊
+  case load₁ IH HEq𝕊 =>
+    rw [escape_meffects.read]
+    apply typing.load₁
+    apply IH; apply HEq𝕊
+  case store₁ IHl IHr HEq𝕊 =>
+    rw [escape_meffects.write]
+    apply typing.store₁
+    . apply IHl; apply HEq𝕊
+    . apply IHr; apply HEq𝕊
+  apply Hτ
+
+theorem typing.escape :
+  ∀ σ e τ φ ω,
+    typing σ ⦰ 𝟚 e τ φ ω →
+    typing σ ⦰ 𝟙 e (escape_ty τ) φ (escape_meffects ω) :=
+  by
+  intros σ e τ φ ω Hτ
+  apply typing.escape.strengthened _ _ _ _ _ _ Hτ
+
+theorem preservation.pure.head :
+  ∀ σ Γ e₀ e₁ τ φ₀ ω₀,
+    head_pure e₀ e₁ →
+    typing σ Γ 𝟙 e₀ τ φ₀ ω₀ →
+    ∃ φ₁ ω₁,
+      typing σ Γ 𝟙 e₁ τ φ₁ ω₁ ∧
+      φ₁ ≤ φ₀ ∧
+      ω₁ ≤ ω₀ :=
+  by
+  intros σ Γ e₀ e₁ τ φ₀ ω₀ Hhead Hτ
+  have Hlc := typing.regular _ _ _ _ _ _ _ Hτ
+  cases Hhead
+  case lets Hvalue =>
+    exists φ₀, ω₀; simp
+    cases Hτ
+    case lets φ₀ φ₁ ω₀ ω₁ _ Hτv Hclosed Hτe =>
+      have Hpureφ : φ₀ = ⊥ := by cases Hvalue <;> cases Hτv <;> rfl
+      have Hpureω : ω₀ = ∅ := by cases Hvalue <;> cases Hτv <;> simp at *
+      simp [Hpureφ, Hpureω] at Hτv
+      simp [Hpureφ, Hpureω]
+      rw [← intro.subst _ _ _ _ Hclosed]
+      apply preservation.subst _ _ _ _ _ _ _ _ _ Hτv Hτe
+  case app₁ Hvalue =>
+    exists φ₀, ω₀; simp
+    cases Hτ
+    case app₁ φ₀ φ₁ φ₂ ω₀ ω₁ ω₂ Hτv Hτf =>
+      cases Hτf
+      case lam Hclosed _ Hτe =>
+        have Hpureφ : φ₂ = ⊥ := by cases Hvalue <;> cases Hτv <;> rfl
+        have Hpureω : ω₂ = ∅ := by cases Hvalue <;> cases Hτv <;> simp at *
+        simp [Hpureφ, Hpureω] at Hτv
+        simp [Hpureφ, Hpureω]
+        rw [← intro.subst _ _ _ _ Hclosed]
+        apply preservation.subst _ _ _ _ _ _ _ _ _ Hτv Hτe
+  case app₂ =>
+    exists φ₀, ω₀; simp
+    cases Hτ
+    case app₂ Hτ₀ Hτ₁ =>
+      cases Hτ₀
+      case code_fragment Hwbt₀ Hbinds₀ =>
+        cases Hτ₁
+        case code_fragment Hwbt₁ Hbinds₁ =>
+          apply typing.reflect
+          rw [← REffects.union_pure ⊥, ← REffects.union_pure (⊥ ∪ ⊥)]
+          apply typing.app₁
+          . apply typing.fvar; apply Hbinds₀; apply Hwbt₀
+          . apply typing.fvar; apply Hbinds₁; apply Hwbt₁
+  case lift_lit =>
+    exists φ₀, ω₀; simp
+    cases Hτ
+    case lift_lit Hτ =>
+      cases Hτ
+      apply typing.reflect
+      apply typing.lit
+    case lift_lam => contradiction
+    case lift_unit => contradiction
+  case lift_lam =>
+    exists φ₀, ω₀; simp
+    cases Hτ
+    case lift_lam Hτ =>
+      cases Hτ
+      case lam Hω Hclosed Hwbt Hτe =>
+        apply typing.lam𝕔
+        . apply typing_reification.reify
+          rw [← intro.codify _ _ _ Hclosed, identity.opening_closing]
+          apply preservation.maping _ _ _ _ _ _ _ _ _ _ Hτe
+          apply typing.code_fragment; simp; apply Hwbt
+          apply lc.under_subst
+          . simp
+          . apply typing.regular _ _ _ _ _ _ _ Hτe
+        . apply Hwbt
+        . rw [← closed.under_codify]; apply Hclosed
+        . apply Hω
+    case lift_lit => contradiction
+    case lift_unit => contradiction
+  case lift_unit =>
+    exists φ₀, ω₀; simp
+    cases Hτ
+    case lift_unit Hτ =>
+      cases Hτ
+      apply typing.reflect
+      apply typing.unit
+    case lift_lit => contradiction
+    case lift_lam => contradiction
+  case lam𝕔 e =>
+    exists φ₀, ω₀; simp
+    cases Hτ
+    case lam𝕔 Hwbt _ Hτ Hclosed =>
+      apply typing.reflect
+      apply typing.lam
+      . apply typing_reification_code _ _ _ _ _ _ Hτ
+      . apply Hwbt
+      . apply Hclosed
+  case lets𝕔 b e =>
+    exists φ₀, ω₀; simp
+    cases Hτ
+    case lets𝕔 Hwbt Hτb Hτe Hclosed =>
+      apply typing.code_rep
+      rw [← REffects.union_pure ⊥]
+      apply typing.lets
+      . apply Hτb
+      . apply typing_reification_code _ _ _ _ _ _ Hτe
+      . apply Hwbt
+      . apply Hclosed
+  case run =>
+    exists φ₀, ω₀; simp
+    cases Hτ
+    case run Hclosed Hτ =>
+      rw [← List.append_nil Γ]
+      apply typing.weakening
+      apply typing.escape
+      apply typing.shrinking; simp
+      apply typing_reification_code _ _ _ _ _ _ Hτ
+      apply Hclosed
+  case alloc₂ Hτ =>
+    exists φ₀, ω₀; simp
+    cases Hτ
+    case alloc₂ Hτ =>
+      cases Hτ
+      case code_fragment Hwbt Hbinds =>
+        apply typing.reflect
+        apply typing.alloc₁
+        apply typing.fvar; apply Hbinds; apply Hwbt
+  case load₂ Hτ =>
+    exists φ₀, ω₀; simp
+    cases Hτ
+    case load₂ Hτ =>
+      cases Hτ
+      case code_fragment Hwbt Hbinds =>
+        apply typing.reflect
+        apply typing.load₁
+        apply typing.fvar; apply Hbinds; apply Hwbt
+  case store₂ Hτ =>
+    exists φ₀, ω₀; simp
+    cases Hτ
+    case store₂ Hτ₀ Hτ₁ =>
+      cases Hτ₀
+      case code_fragment Hwbt₀ Hbinds₀ =>
+        cases Hτ₁
+        case code_fragment Hwbt₁ Hbinds₁ =>
+          apply typing.reflect
+          rw [← REffects.union_pure ⊥]
+          apply typing.store₁
+          . apply typing.fvar; apply Hbinds₀; apply Hwbt₀
+          . apply typing.fvar; apply Hbinds₁; apply Hwbt₁
+
+theorem preservation.pure :
+  ∀ σ Γ M e₀ e₁ τ φ₀ ω₀,
+    ctx𝕄 Γ.length M →
+    lc e₀ →
+    head_pure e₀ e₁ →
+    typing σ Γ 𝟙 M⟦e₀⟧ τ φ₀ ω₀ →
+    ∃ φ₁ ω₁,
+      typing σ Γ 𝟙 M⟦e₁⟧ τ φ₁ ω₁ ∧
+      φ₁ ≤ φ₀ ∧
+      ω₁ ≤ ω₀ :=
+  by
+  intros σ Γ M e₀ e₁ τ φ₀ ω₀ HM Hlc Hhead Hτ
+  generalize HEqlvl : Γ.length = lvl
+  rw [HEqlvl] at HM
+  induction HM generalizing Γ τ φ₀ ω₀
+  case hole => apply preservation.pure.head _ _ _ _ _ _ _ Hhead Hτ
+  case cons𝔹 B M HB HM IH =>
+    have ⟨τ𝕖, φ₁, φ₂, ω₁, ω₂, HEqφ, HEqω, Hτ, IHτB⟩ := preservation.under_ctx𝔹 _ _ _ _ _ _ _ HB Hτ
+    rw [HEqφ, HEqω]
+    have ⟨φ₃, ω₃, Hτ, HLeφ, HLeω⟩ := IH _ _ _ _ Hτ HEqlvl
+    have Hτ := IHτB σ ⦰ _ _ _ (by omega) Hτ
+    exists φ₃ ∪ φ₂, ω₃ ∪ ω₂; constructor
+    . apply Hτ
+    . constructor
+      . cases φ₁ <;> cases φ₂ <;> cases φ₃ <;> simp at HLeφ <;> simp
+      . apply Set.union_subset_union_left _ HLeω
+  case consℝ R M HR HM IH =>
+    admit
